Hiding game Def

KZG_hiding.thy
@@ -21,6 +21,11 @@ not really fit as we are not trying to come up with two different plain texts bu
 \<close>
 text \<open>The evaluation commitment scheme functions.\<close>
 
+(*TODO delete*)
+thm ennreal_spmf_bind
+thm spmf_bind
+thm nn_integral_measure_spmf
+
 text \<open>Expose just the public key from the Setup\<close>
 definition key_gen:: "'a pk spmf" where
   "key_gen = do {
@@ -37,19 +42,17 @@ type_synonym ('a', 'e')  adversary =
   "'a' commit \<Rightarrow> ('e' eval_position \<times> 'e' eval_value \<times> 'a' eval_witness) list \<Rightarrow> 
  'e' polynomial spmf"
 
-definition hiding_Adversary_game :: "'e mod_ring \<Rightarrow> 'e eval_position list \<Rightarrow> 'e polynomial \<Rightarrow> ('a, 'e) adversary \<Rightarrow> bool spmf"
-  where "hiding_Adversary_game \<alpha> eval_pos \<phi> \<A> = do {
-  let PK = map (\<lambda>t. \<^bold>g\<^bsub>G\<^sub>p\<^esub> ^\<^bsub>G\<^sub>p\<^esub> (\<alpha>^t)) [0..<max_deg+1];
+definition hiding_game :: "'e eval_position list \<Rightarrow> ('a, 'e) adversary \<Rightarrow> bool spmf"
+  where "hiding_game I \<A> = TRY do {
+  \<phi> \<leftarrow> sample_uniform_poly max_deg;
+  PK \<leftarrow> key_gen;
   let C = Commit PK \<phi>;
-  let witn_tupel = map (\<lambda>i. (i, poly \<phi> i, createWitness PK \<phi> i)) eval_pos;
-  \<phi>' \<leftarrow> \<A> C witn_tupel;
-  _ :: unit \<leftarrow> assert_spmf (\<phi> = \<phi>');
-  return_spmf True}"
+  let witn_tupel = map (\<lambda>i. (i, poly \<phi> i, createWitness PK \<phi> i)) I;
+  \<phi>' \<leftarrow> \<A> C witn_tupel;                             
+  return_spmf (\<phi> = \<phi>')} ELSE return_spmf False"
 
-text \<open>put C and eval_poses in parameter and assert\<close>
-
-definition hiding_advantage :: "'e mod_ring \<Rightarrow> 'e eval_position list \<Rightarrow>  'e polynomial \<Rightarrow> ('a, 'e) adversary \<Rightarrow> real"
-  where "hiding_advantage \<alpha> eval_pos \<phi> \<A> \<equiv> spmf (hiding_Adversary_game \<alpha> eval_pos \<phi> \<A>) True"
+definition hiding_advantage :: "'e eval_position list \<Rightarrow> ('a, 'e) adversary \<Rightarrow> real"
+  where "hiding_advantage I \<A> \<equiv> spmf (hiding_game I \<A>) True"
 
 subsection \<open>DL game\<close>
 
@@ -59,26 +62,33 @@ sublocale DL_G\<^sub>p: DL G\<^sub>p "of_int_mod_ring \<circ> int" "pow_mod_ring
 
 subsection \<open>Reduction\<close>
 
-lemma split_sample_distinct_coordinates_uniform_into_points:
-"bind_spmf (sample_distinct_coordinates_uniform k n) (\<lambda>coords. return_spmf coords) =
-  do {
-   points \<leftarrow> sample_distinct_uniform_list k n;
-   coords \<leftarrow> map_spmf pair_lists (pair_spmf (return_spmf points) (sample_uniform_list k n));
-   return_spmf coords
+definition compute_g_pow_\<phi>_of_\<alpha> :: "('e mod_ring \<times> 'a) list \<Rightarrow> 'e mod_ring \<Rightarrow> 'a" where
+  "compute_g_pow_\<phi>_of_\<alpha> xs_ys \<alpha>= do {
+  let xs = map fst xs_ys;
+  let lagrange_exp = map (\<lambda>(xj,yj). yj ^\<^bsub>G\<^sub>p\<^esub> (poly (lagrange_basis_poly xs xj) \<alpha>)) xs_ys;
+  fold (\<lambda>x prod. prod \<otimes>\<^bsub>G\<^sub>p\<^esub> x) lagrange_exp \<one>}"
+
+fun reduction
+  :: "'e eval_position list \<Rightarrow> ('a, 'e) adversary \<Rightarrow> ('a,'e) DL.adversary"                     
+where
+  "reduction I \<A> g_pow_a = do {
+  evals \<leftarrow> sample_uniform_list (max_deg-1) (order G\<^sub>p);
+  let exp_evals = map (\<lambda>i. \<^bold>g [^] i) evals ;
+  (\<alpha>, PK) \<leftarrow> Setup;
+  let C = compute_g_pow_\<phi>_of_\<alpha> (zip I exp_evals) \<alpha>;
+  let wtn_ts = map (\<lambda>(x,y). (x,y,(C  \<div>\<^bsub>G\<^sub>p\<^esub> \<^bold>g\<^bsub>G\<^sub>p\<^esub> ^\<^bsub>G\<^sub>p\<^esub> y) ^\<^bsub>G\<^sub>p\<^esub> (1/(\<alpha>-x)))) (zip (tl I) (map (of_int_mod_ring \<circ> int) evals));
+  \<phi>' \<leftarrow> \<A> C wtn_ts;
+  return_spmf (poly \<phi>' (hd I))
   }"
-  unfolding sample_distinct_coordinates_uniform_def 
-  by (smt (verit) bind_return_spmf bind_spmf_cong map_spmf_bind_spmf pair_spmf_alt_def return_bind_spmf)
 
-(* TODO delete +  lemma after this*)
-definition sample_n_coords :: "nat \<Rightarrow> ('e mod_ring \<times> 'e mod_ring) list spmf"
-where 
-  "sample_n_coords n =
-    map_spmf (map (\<lambda>(x,y). (of_int_mod_ring (int x),of_int_mod_ring (int y))))
-    (sample_distinct_coordinates_uniform n (order G\<^sub>p))"
+end 
 
-lemma length_pair_lists: "length xs = n \<Longrightarrow> length ys = n \<Longrightarrow> length (pair_lists (xs,ys)) = n"
-  by (induction "(xs,ys)" arbitrary: n xs ys rule: pair_lists.induct)simp+
+locale hiding_game_proof = hiding_game_def 
+begin
 
+subsection \<open>Reduction proof\<close>
+
+subsubsection \<open>helping lemmas\<close>
 
 lemma eval_on_lagrange_basis: "poly (lagrange_interpolation_poly xs_ys) x \<equiv> (let 
     xs = map fst xs_ys
@@ -120,12 +130,6 @@ next
      using G\<^sub>p.cyclic_group_assoc mod_ring_pow_mult_G\<^sub>p by force
    finally show ?case .
  qed
-
-definition compute_g_pow_\<phi>_of_\<alpha> :: "('e mod_ring \<times> 'a) list \<Rightarrow> 'e mod_ring \<Rightarrow> 'a" where
-  "compute_g_pow_\<phi>_of_\<alpha> xs_ys \<alpha>= do {
-  let xs = map fst xs_ys;
-  let lagrange_exp = map (\<lambda>(xj,yj). yj ^\<^bsub>G\<^sub>p\<^esub> (poly (lagrange_basis_poly xs xj) \<alpha>)) xs_ys;
-  fold (\<lambda>x prod. prod \<otimes>\<^bsub>G\<^sub>p\<^esub> x) lagrange_exp \<one>}"
 
 lemma compute_g_pow_\<phi>_of_\<alpha>_is_Commit:
   assumes dist: "distinct (map fst xs_ys)"
@@ -233,25 +237,6 @@ proof -
     by fast
 qed
 
-
-fun reduction
-  :: "('a, 'e) adversary \<Rightarrow> ('a,'e) DL.adversary"                     
-where
-  "reduction \<A> g_pow_a = do {
-    let coords = zip (map (of_int_mod_ring \<circ> int) [0..<max_deg + 1]) (map (of_int_mod_ring \<circ> int) [0..<max_deg + 1]); 
-    let exp_coords = (fst (hd coords),g_pow_a)#map (\<lambda>(x,y). (x,\<^bold>g\<^bsub>G\<^sub>p\<^esub> ^\<^bsub>G\<^sub>p\<^esub> y)) (tl coords);
-    (\<alpha>, PK) \<leftarrow> Setup;
-    let g_pow_\<phi>_of_\<alpha> = compute_g_pow_\<phi>_of_\<alpha> exp_coords \<alpha>;
-    let wtn_tuples = map (\<lambda>(x,y). (x,y,(g_pow_\<phi>_of_\<alpha>  \<div>\<^bsub>G\<^sub>p\<^esub> \<^bold>g\<^bsub>G\<^sub>p\<^esub> ^\<^bsub>G\<^sub>p\<^esub> y) ^\<^bsub>G\<^sub>p\<^esub> (1/(\<alpha>-x)))) (tl coords);
-    \<phi>' \<leftarrow> \<A> g_pow_\<phi>_of_\<alpha> wtn_tuples;
-    return_spmf (poly \<phi>' 0)}"
-
-(*sample n coords max_deg + 1 (for point (x,a) ) *)
-
-subsection \<open>Reduction proof\<close>
-
-subsubsection \<open>helping lemmas\<close>
-
 lemma of_int_mod_inj_on_ff: "inj_on (of_int_mod_ring \<circ> int:: nat \<Rightarrow> 'e mod_ring) {0..<CARD ('e)}"
 proof 
   fix x 
@@ -263,140 +248,13 @@ proof
     using x y app_x_eq_y 
     by (metis atLeastLessThan_iff nat_int o_apply of_nat_0_le_iff of_nat_less_iff to_int_mod_ring_of_int_mod_ring)
 qed
-    
-
-lemma literal_helping_1: 
-  assumes "max_deg + 1 < CARD ('e)"
-  shows "(let coords = zip (map (of_int_mod_ring \<circ> int:: nat \<Rightarrow> 'e mod_ring) [0..<max_deg + 1]) (map (of_int_mod_ring \<circ> int:: nat \<Rightarrow> 'e mod_ring) [0..<max_deg + 1]);
-        exp_coords = (fst (hd coords),(\<^bold>g ^\<^bsub>G\<^sub>p\<^esub> a))#map (\<lambda>(x,y). (x,\<^bold>g\<^bsub>G\<^sub>p\<^esub> ^\<^bsub>G\<^sub>p\<^esub> y)) (tl coords) in 
-  compute_g_pow_\<phi>_of_\<alpha> exp_coords \<alpha> 
-  = Commit (map (\<lambda>t. \<^bold>g\<^bsub>G\<^sub>p\<^esub> ^\<^bsub>G\<^sub>p\<^esub> (\<alpha>^t)) [0..<max_deg+1]) (lagrange_interpolation_poly ((fst (hd coords),a)#tl coords)))"
-proof -
-  let ?coords = "zip (map (of_int_mod_ring \<circ> int:: nat \<Rightarrow> 'e mod_ring) [0..<max_deg + 1]) (map (of_int_mod_ring \<circ> int:: nat \<Rightarrow> 'e mod_ring) [0..<max_deg + 1])::('e mod_ring*'e mod_ring) list"
-  let ?exp_coords = "(fst (hd ?coords),(\<^bold>g ^\<^bsub>G\<^sub>p\<^esub> a))#map (\<lambda>(x,y). (x,\<^bold>g\<^bsub>G\<^sub>p\<^esub> ^\<^bsub>G\<^sub>p\<^esub> y)) (tl ?coords)"
-  let ?PK = "(map (\<lambda>t. \<^bold>g\<^bsub>G\<^sub>p\<^esub> ^\<^bsub>G\<^sub>p\<^esub> (\<alpha>^t)) [0..<max_deg+1])"
-
-  have "compute_g_pow_\<phi>_of_\<alpha> ?exp_coords \<alpha> = Commit ?PK (lagrange_interpolation_poly ((fst (hd ?coords), a)#tl ?coords))"
-  proof -
-    obtain xs_ys where xs_ys: "xs_ys = (fst (hd ?coords),a)#tl ?coords" by fast
-    then have exp_coords_is_map_xs_ys: "?exp_coords = (map (\<lambda>(x, y). (x, \<^bold>g ^\<^bsub>G\<^sub>p\<^esub> y)) xs_ys)" by force
-    from xs_ys have dist_xs_ys: "distinct (map fst xs_ys)"
-    proof -
-      have "(map fst xs_ys) = (map (of_int_mod_ring \<circ> int) [0..<max_deg + 1])"
-      proof -
-        have "map fst ((fst (hd ?coords),a)#tl ?coords) = fst (fst (hd ?coords),a) # map fst (tl ?coords)"
-          by force
-        also have "\<dots> = fst (hd ?coords) # map fst (tl ?coords)"
-          by fastforce
-        also have "\<dots> = map fst (?coords)"
-          by (simp add: d_pos hd_zip map_tl)
-        also have "\<dots> = map (of_int_mod_ring \<circ> int:: nat \<Rightarrow> 'e mod_ring) [0..<max_deg + 1]"
-          by force
-        finally show ?thesis unfolding xs_ys .
-      qed
-      moreover have "distinct (map (of_int_mod_ring \<circ> int:: nat \<Rightarrow> 'e mod_ring) [0..<max_deg + 1])"
-      proof -
-        have "distinct [0..<max_deg + 1]"
-          by auto
-        moreover have "inj_on (of_int_mod_ring \<circ> int:: nat \<Rightarrow> 'e mod_ring) (set [0..<max_deg + 1])"
-        proof - 
-          have "(set [0..<max_deg + 1]) \<subseteq> {0..<CARD ('e)}"
-            using assms by auto
-          then show ?thesis 
-            using of_int_mod_inj_on_ff inj_on_subset by blast 
-        qed
-        ultimately show ?thesis
-          using distinct_map[of "(of_int_mod_ring \<circ> int)" "[0..<max_deg + 1]"] by blast
-      qed
-      ultimately show ?thesis by argo
-    qed
-    moreover have length_xs_ys: "length xs_ys \<le> max_deg +1"
-    proof -
-      have "length xs_ys = length ?coords"
-        unfolding xs_ys 
-        by force
-      also have "\<dots> = max_deg +1"
-        by fastforce
-      finally show ?thesis by simp
-    qed
-    show ?thesis using compute_g_pow_\<phi>_of_\<alpha>_is_Commit[OF dist_xs_ys length_xs_ys]
-      unfolding xs_ys
-      by fastforce
-  qed
-  then show ?thesis unfolding Let_def .
-qed
 
 subsubsection \<open>reduction proof\<close>
 
-thm ennreal_spmf_bind
 
-thm spmf_bind
-thm nn_integral_measure_spmf
-
-   declare [[show_types]] 
-theorem
-  assumes "max_deg + 1 < CARD ('e)"
-  shows "spmf (DL_G\<^sub>p.game (reduction \<A>)) True = 1"
-proof -
-  note [simp] = Let_def split_def
-  let ?mr = "\<lambda>\<alpha>. (of_int_mod_ring (int \<alpha>)::'e mod_ring)"
-  have "DL_G\<^sub>p.game (reduction \<A>) = TRY do {
-      a \<leftarrow> sample_uniform (order G\<^sub>p);
-      let eval_pos = map (?mr) [order G\<^sub>p - max_deg + 1..<order G\<^sub>p];
-      \<alpha> \<leftarrow> sample_uniform (order G\<^sub>p - max_deg);
-      let coords = (?mr (order G\<^sub>p - max_deg), (?mr a))#zip eval_pos eval_pos;
-      hiding_Adversary_game (?mr \<alpha>) eval_pos (lagrange_interpolation_poly coords) \<A>
-    } ELSE return_spmf False"
-    sorry
-  then have "spmf (DL_G\<^sub>p.game (reduction \<A>)) True = spmf (TRY do {
-      a \<leftarrow> sample_uniform (order G\<^sub>p);
-      let eval_pos = map (?mr) [order G\<^sub>p - max_deg + 1..<order G\<^sub>p];
-      \<alpha> \<leftarrow> sample_uniform (order G\<^sub>p - max_deg);
-      let coords = (?mr (order G\<^sub>p - max_deg), (?mr a))#zip eval_pos eval_pos;
-      hiding_Adversary_game (?mr \<alpha>) eval_pos (lagrange_interpolation_poly coords) \<A>
-    } ELSE return_spmf False) True"
-    by presburger
-  also have "\<dots> = spmf (do {
-      a \<leftarrow> sample_uniform (order G\<^sub>p);
-      let eval_pos = map (?mr) [order G\<^sub>p - max_deg + 1..<order G\<^sub>p];
-      \<alpha> \<leftarrow> sample_uniform (order G\<^sub>p - max_deg);
-      let coords = (?mr (order G\<^sub>p - max_deg), (?mr a))#zip eval_pos eval_pos;
-      hiding_Adversary_game (?mr \<alpha>) eval_pos (lagrange_interpolation_poly coords) \<A>
-    }) True"
-    unfolding spmf_try_spmf
-    by force
-  also have "\<dots> = (\<Sum>\<^sup>+ x. ennreal (spmf (sample_uniform (order G\<^sub>p)) x) * spmf
-        (do {let eval_pos = map ?mr [order G\<^sub>p - max_deg + 1..<order G\<^sub>p];
-             \<alpha> \<leftarrow> sample_uniform (order G\<^sub>p - max_deg);
-            let coords =(?mr (order G\<^sub>p - max_deg), ?mr x) # zip eval_pos eval_pos;
-            hiding_Adversary_game (?mr \<alpha>) eval_pos (lagrange_interpolation_poly coords) \<A>})
-        True)"
-    unfolding ennreal_spmf_bind nn_integral_measure_spmf ..
-  moreover have "\<dots> = 1/real (order G\<^sub>p) * (\<Sum> x<order G\<^sub>p. spmf
-        (do {let eval_pos = map ?mr [order G\<^sub>p - max_deg + 1..<order G\<^sub>p];
-             \<alpha> \<leftarrow> sample_uniform (order G\<^sub>p - max_deg);
-            let coords =(?mr (order G\<^sub>p - max_deg), ?mr x) # zip eval_pos eval_pos;
-            hiding_Adversary_game (?mr \<alpha>) eval_pos (lagrange_interpolation_poly coords) \<A>})
-        True)"
-    unfolding spmf_sample_uniform sorry
-  moreover have "\<dots> = 1/real (order G\<^sub>p) * 1/real (order G\<^sub>p - max_deg) * (\<Sum> \<alpha><order G\<^sub>p- max_deg. \<Sum> x<order G\<^sub>p. spmf
-        (do {let eval_pos = map ?mr [order G\<^sub>p - max_deg + 1..<order G\<^sub>p];
-            let coords =(?mr (order G\<^sub>p - max_deg), ?mr x) # zip eval_pos eval_pos;
-            hiding_Adversary_game (?mr \<alpha>) eval_pos (lagrange_interpolation_poly coords) \<A>})
-        True)"
-    unfolding spmf_sample_uniform sorry
-
-      
   
-    
   
-
-  show ?thesis
-  using assms unfolding DL_G\<^sub>p.game_def reduction.simps
-  key_gen_def Let_def Setup_def
-  sorry
-qed
-
+  
 end
 
 
